<?xml version="1.0"?>
<rdf:RDF xmlns:rdfs="http://www.w3.org/2000/01/rdf-schema#" xmlns:xsd="http://www.w3.org/2001/XMLSchema#" xmlns:dc="http://purl.org/dc/elements/1.1/" xmlns:owl="http://www.w3.org/2002/07/owl#" xmlns:rdf="http://www.w3.org/1999/02/22-rdf-syntax-ns#">
	<owl:Ontology rdf:about="http://dkm.fbk.eu/springles/ruleset#">
		<owl:versionInfo>0.1</owl:versionInfo>
		<dc:title xml:lang="en">Springles Ruleset Vocabulary</dc:title>
		<dc:rights xml:lang="en">Copyright &amp;#169; 2013 FBK-Irst</dc:rights>
		<dc:creator rdf:resource="https://dkm.fbk.eu/index.php/Luciano_Serafini" />
		<dc:creator rdf:resource="https://dkm.fbk.eu/index.php/Loris_Bozzato" />
		<dc:creator rdf:resource="https://dkm.fbk.eu/index.php/Francesco_Corcoglioniti" />
	</owl:Ontology>
	<owl:Class rdf:about="http://dkm.fbk.eu/springles/ruleset#Ruleset">
		<rdfs:label xml:lang="en">ruleset</rdfs:label>
		<rdfs:comment xml:lang="en">A ruleset consists of a set of rules, evaluated either in
        backward- or forward- chaining. Backward evaluation (currently
        unsupported) affects rules listed by property
        &lt;a href='#evalBackward'&gt;spr:evalBackward&lt;/a&gt;. Forward evaluation is
        specified by supplying a closure plan with property
        &lt;a href='#closurePlan'&gt;spr:closurePlan&lt;/a&gt;. A ruleset is optionally
        associated to a number of ruleset parameters via property
        &lt;a href='#parameterizedBy'&gt;spr:parameterizedBy&lt;/a&gt;, a 'SPARQL prologue'
        via property &lt;a href='#prologue'&gt;spr:prologue&lt;/a&gt; and a number of
        'macros' via property &lt;a href='#macro'&gt;spr:macro&lt;/a&gt;.</rdfs:comment>
		<rdfs:subClassOf>
			<owl:Restriction>
				<owl:onProperty>
					<owl:ObjectProperty rdf:about="http://dkm.fbk.eu/springles/ruleset#closurePlan">
						<rdf:type rdf:resource="http://www.w3.org/2002/07/owl#FunctionalProperty" />
						<rdfs:label xml:lang="en">closure plan</rdfs:label>
						<rdfs:comment xml:lang="en">Specifies the mandatory closure plan associated to the 
        ruleset.</rdfs:comment>
						<rdfs:domain rdf:resource="http://dkm.fbk.eu/springles/ruleset#Ruleset" />
						<rdfs:range>
							<owl:Class rdf:about="http://dkm.fbk.eu/springles/ruleset#ClosureTask">
								<rdfs:label xml:lang="en">closure task</rdfs:label>
								<rdfs:comment xml:lang="en">A generic task of the closure plan. Explicit definition of
        variable bindings is supported for any type of task using property
        &lt;a href='#bind'&gt;spr:bind&lt;/a&gt;.</rdfs:comment>
							</owl:Class>
						</rdfs:range>
					</owl:ObjectProperty>
				</owl:onProperty>
				<owl:minCardinality rdf:datatype="http://www.w3.org/2001/XMLSchema#nonNegativeInteger">1</owl:minCardinality>
			</owl:Restriction>
		</rdfs:subClassOf>
	</owl:Class>
	<owl:ObjectProperty rdf:about="http://dkm.fbk.eu/springles/ruleset#parameterizedBy">
		<rdfs:label xml:lang="en">parameterized by</rdfs:label>
		<rdfs:comment xml:lang="en">Specifies the (optional) parameters of the ruleset.</rdfs:comment>
		<rdfs:domain rdf:resource="http://dkm.fbk.eu/springles/ruleset#Ruleset" />
		<rdfs:range>
			<owl:Class rdf:about="http://dkm.fbk.eu/springles/ruleset#Parameter">
				<rdfs:label xml:lang="en">parameter</rdfs:label>
				<rdfs:comment xml:lang="en">A ruleset parameter characterized by a name (property
        &lt;a href='#name'&gt;spr:name&lt;/a&gt;) and a default value (property
        &lt;a href='#default'&gt;spr:default&lt;/a&gt;), whose value may be supplied by
        users at repository configuration time.</rdfs:comment>
				<rdfs:subClassOf>
					<owl:Restriction>
						<owl:onProperty>
							<owl:DatatypeProperty rdf:about="http://dkm.fbk.eu/springles/ruleset#name">
								<rdf:type rdf:resource="http://www.w3.org/2002/07/owl#FunctionalProperty" />
								<rdfs:label xml:lang="en">name</rdfs:label>
								<rdfs:comment xml:lang="en">Specifies the name of a ruleset parameter.</rdfs:comment>
								<rdfs:domain rdf:resource="http://dkm.fbk.eu/springles/ruleset#Parameter" />
								<rdfs:range rdf:resource="http://www.w3.org/2001/XMLSchema#string" />
							</owl:DatatypeProperty>
						</owl:onProperty>
						<owl:minCardinality rdf:datatype="http://www.w3.org/2001/XMLSchema#nonNegativeInteger">1</owl:minCardinality>
					</owl:Restriction>
				</rdfs:subClassOf>
				<rdfs:subClassOf>
					<owl:Restriction>
						<owl:onProperty>
							<owl:DatatypeProperty rdf:about="http://dkm.fbk.eu/springles/ruleset#default">
								<rdfs:label xml:lang="en">default value</rdfs:label>
								<rdfs:comment xml:lang="en">Specifies the default value of a parameter. Literal values
        of type xsd:anyURI are injected as IRIs (instead of literals) in
        SPARQL expressions.</rdfs:comment>
								<rdfs:domain rdf:resource="http://dkm.fbk.eu/springles/ruleset#LiteralParameter" />
								<rdfs:range rdf:resource="http://www.w3.org/2000/01/rdf-schema#Literal" />
							</owl:DatatypeProperty>
						</owl:onProperty>
						<owl:minCardinality rdf:datatype="http://www.w3.org/2001/XMLSchema#nonNegativeInteger">1</owl:minCardinality>
					</owl:Restriction>
				</rdfs:subClassOf>
			</owl:Class>
		</rdfs:range>
	</owl:ObjectProperty>
	<owl:DatatypeProperty rdf:about="http://dkm.fbk.eu/springles/ruleset#prologue">
		<rdf:type rdf:resource="http://www.w3.org/2002/07/owl#FunctionalProperty" />
		<rdfs:label xml:lang="en">prologue</rdfs:label>
		<rdfs:comment xml:lang="en">Specifies the optional SPARQL prologue, consisting of
        namespace declarations (syntax &lt;code&gt;PREFIX pref: &amp;lt;uri&amp;gt;&gt;&lt;/code&gt;)
        and base URI declaration (syntax &lt;code&gt;BASE &amp;lt;uri&amp;gt;&gt;&lt;/code&gt;).
        </rdfs:comment>
		<rdfs:domain rdf:resource="http://dkm.fbk.eu/springles/ruleset#Ruleset" />
		<rdfs:range rdf:resource="http://www.w3.org/2001/XMLSchema#string" />
	</owl:DatatypeProperty>
	<owl:DatatypeProperty rdf:about="http://dkm.fbk.eu/springles/ruleset#macro">
		<rdfs:label xml:lang="en">macro</rdfs:label>
		<rdfs:comment xml:lang="en">Defines a macro using syntax
        &lt;code&gt;macro(arg1, ..., argN) = template&lt;/code&gt;. Arguments are optional,
        in which case parenthesis can be omitted. Arguments can be referenced in
        the template with the syntax &lt;code&gt;#arg&lt;/code&gt;. As a safety measure, if
        an argument &lt;code&gt;arg&lt;/code&gt; is defined, no SPARQL variable
        &lt;code&gt;?arg&lt;/code&gt; can be used in the template. Macros can be used in
        SPARQL expressions being the objects of &lt;a href='#head'&gt;spr:head&lt;/a&gt;,
        &lt;a href='#body'&gt;spr:body&lt;/a&gt;, &lt;a href='#condition'&gt;spr:condition&lt;/a&gt; and
        &lt;a href='#bind'&gt;spr:bind&lt;/a&gt; properties.</rdfs:comment>
		<rdfs:domain rdf:resource="http://dkm.fbk.eu/springles/ruleset#Ruleset" />
		<rdfs:range rdf:resource="http://www.w3.org/2001/XMLSchema#string" />
	</owl:DatatypeProperty>
	<owl:ObjectProperty rdf:about="http://dkm.fbk.eu/springles/ruleset#evalBackward">
		<rdfs:label xml:lang="en">eval backward</rdfs:label>
		<rdfs:comment xml:lang="en">Specifies the rules to be evaluated in backward-chaining.
        Note that forward- and backward- evaluation of a rule are mutually
        exclusive.</rdfs:comment>
		<owl:propertyDisjointWith>
			<owl:ObjectProperty rdf:about="http://dkm.fbk.eu/springles/ruleset#evalForward">
				<rdfs:label xml:lang="en">eval forward</rdfs:label>
				<rdfs:comment xml:lang="en">Specifies the rules to be evaluated in a forward-chaining
        mode. If a closure plan is supplied, then this property can be omitted;
        otherwise, the rules listed here are evaluated according to a basic plan
        performing fix-point evaluation of all forward-chanining rules.</rdfs:comment>
				<owl:propertyDisjointWith rdf:resource="http://dkm.fbk.eu/springles/ruleset#evalBackward" />
				<rdfs:domain rdf:resource="http://dkm.fbk.eu/springles/ruleset#Ruleset" />
				<rdfs:range rdf:resource="http://dkm.fbk.eu/springles/ruleset#Rule" />
			</owl:ObjectProperty>
		</owl:propertyDisjointWith>
		<rdfs:domain rdf:resource="http://dkm.fbk.eu/springles/ruleset#Ruleset" />
		<rdfs:range>
			<owl:Class rdf:about="http://dkm.fbk.eu/springles/ruleset#Rule">
				<rdfs:label xml:lang="en">rule</rdfs:label>
				<rdfs:comment xml:lang="en">An inference rule expressed using SPARQL, with mandatory
        &lt;a href='#head'&gt;spr:head&lt;/a&gt; and &lt;a href='#body'&gt;spr:body&lt;/a&gt;, and
        optional &lt;a href='#condition'&gt;spr:condition&lt;/a&gt;, transformer (property
        &lt;a href='#transform'&gt;spr:transform&lt;/a&gt;) and list of triggered rules
        (property &lt;a href='#triggerOf'&gt;spr:triggerOf&lt;/a&gt;).</rdfs:comment>
				<rdfs:subClassOf>
					<owl:Restriction>
						<owl:onProperty>
							<owl:DatatypeProperty rdf:about="http://dkm.fbk.eu/springles/ruleset#head">
								<rdf:type rdf:resource="http://www.w3.org/2002/07/owl#FunctionalProperty" />
								<rdfs:label xml:lang="en">head</rdfs:label>
								<rdfs:comment xml:lang="en">Specifies the head of the rule. The value is a SPARQL
        &lt;a href='http://www.w3.org/TR/sparql11-query/#rGroupGraphPattern'&gt;
        spr:GroupGraphPattern&lt;/a&gt; restricted to triple patterns and the
        &lt;code&gt;GRAPH&lt;/code&gt; keyword.</rdfs:comment>
								<rdfs:domain rdf:resource="http://dkm.fbk.eu/springles/ruleset#Rule" />
								<rdfs:range rdf:resource="http://www.w3.org/2001/XMLSchema#string" />
							</owl:DatatypeProperty>
						</owl:onProperty>
						<owl:cardinality rdf:datatype="http://www.w3.org/2001/XMLSchema#nonNegativeInteger">1</owl:cardinality>
					</owl:Restriction>
				</rdfs:subClassOf>
				<rdfs:subClassOf>
					<owl:Restriction>
						<owl:onProperty>
							<owl:DatatypeProperty rdf:about="http://dkm.fbk.eu/springles/ruleset#body">
								<rdf:type rdf:resource="http://www.w3.org/2002/07/owl#FunctionalProperty" />
								<rdfs:label xml:lang="en">body</rdfs:label>
								<rdfs:comment xml:lang="en">Specifies the body of the rule. The value is a SPARQL
        &lt;a href='http://www.w3.org/TR/sparql11-query/#rGroupGraphPattern'&gt;
        spr:GroupGraphPattern&lt;/a&gt;.</rdfs:comment>
								<rdfs:domain rdf:resource="http://dkm.fbk.eu/springles/ruleset#Rule" />
								<rdfs:range rdf:resource="http://www.w3.org/2001/XMLSchema#string" />
							</owl:DatatypeProperty>
						</owl:onProperty>
						<owl:cardinality rdf:datatype="http://www.w3.org/2001/XMLSchema#nonNegativeInteger">1</owl:cardinality>
					</owl:Restriction>
				</rdfs:subClassOf>
			</owl:Class>
		</rdfs:range>
	</owl:ObjectProperty>
	<owl:Class rdf:about="http://dkm.fbk.eu/springles/ruleset#RuleList">
		<rdfs:label xml:lang="en">rule list</rdfs:label>
		<rdfs:comment xml:lang="en">A (possibly empty) list of rules, defined by specializing
        and constraining a generic RDF list.</rdfs:comment>
		<rdfs:subClassOf rdf:resource="http://www.w3.org/1999/02/22-rdf-syntax-ns#List" />
		<rdfs:subClassOf>
			<owl:Restriction>
				<owl:onProperty rdf:resource="http://www.w3.org/1999/02/22-rdf-syntax-ns#first" />
				<owl:allValuesFrom rdf:resource="http://dkm.fbk.eu/springles/ruleset#Rule" />
			</owl:Restriction>
		</rdfs:subClassOf>
		<rdfs:subClassOf>
			<owl:Restriction>
				<owl:onProperty rdf:resource="http://www.w3.org/1999/02/22-rdf-syntax-ns#rest" />
				<owl:allValuesFrom rdf:resource="http://dkm.fbk.eu/springles/ruleset#RuleList" />
			</owl:Restriction>
		</rdfs:subClassOf>
	</owl:Class>
	<owl:DatatypeProperty rdf:about="http://dkm.fbk.eu/springles/ruleset#condition">
		<rdf:type rdf:resource="http://www.w3.org/2002/07/owl#FunctionalProperty" />
		<rdfs:label xml:lang="en">condition</rdfs:label>
		<rdfs:comment xml:lang="en">Specifies the optional rule condition. The value is a SPARQL
        boolean expression satisfying the grammar production
        &lt;a href='http://www.w3.org/TR/sparql11-query/#rConstraint'&gt;
        spr:Constraint&lt;/a&gt;. The expression is evaluated only considering inherited
        variable bindings.</rdfs:comment>
		<rdfs:domain rdf:resource="http://dkm.fbk.eu/springles/ruleset#Rule" />
		<rdfs:range rdf:resource="http://www.w3.org/2001/XMLSchema#string" />
	</owl:DatatypeProperty>
	<owl:DatatypeProperty rdf:about="http://dkm.fbk.eu/springles/ruleset#transform">
		<rdf:type rdf:resource="http://www.w3.org/2002/07/owl#FunctionalProperty" />
		<rdfs:label xml:lang="en">transform</rdfs:label>
		<rdfs:comment xml:lang="en">Specifies the optional transformer associated to the rule.
        The value is a SPARQL
        &lt;a href='http://www.w3.org/TR/sparql11-query/#rFunctionCall'&gt;
        spr:FunctionCall&lt;/a&gt; expression whose URI is the transformer URI (either
        &lt;code&gt;&amp;lt;springles:builtin_function&amp;gt;&lt;/code&gt; or
        &lt;code&gt;&amp;lt;java:class_name.method_name&amp;gt;&lt;/code&gt;) and arguments are
        evaluated based only on inherited variable bindings.</rdfs:comment>
		<rdfs:domain rdf:resource="http://dkm.fbk.eu/springles/ruleset#Rule" />
		<rdfs:range rdf:resource="http://www.w3.org/2001/XMLSchema#string" />
	</owl:DatatypeProperty>
	<owl:ObjectProperty rdf:about="http://dkm.fbk.eu/springles/ruleset#triggerOf">
		<rdfs:label xml:lang="en">trigger of</rdfs:label>
		<rdfs:comment xml:lang="en">Specifies the (possibly empty) list of rule(s) that may fire
        if the subject rule is fired. The property is optional and the order of
        rules in the list is irrelevant.</rdfs:comment>
		<rdfs:domain rdf:resource="http://dkm.fbk.eu/springles/ruleset#Rule" />
		<rdfs:range rdf:resource="http://dkm.fbk.eu/springles/ruleset#RuleList" />
	</owl:ObjectProperty>
	<owl:Class rdf:about="http://dkm.fbk.eu/springles/ruleset#ClosureTaskList">
		<rdfs:label xml:lang="en">closure task list</rdfs:label>
		<rdfs:comment xml:lang="en">A list of closure tasks, defined by specializing and
        constraining a generic RDF list.</rdfs:comment>
		<rdfs:subClassOf rdf:resource="http://www.w3.org/1999/02/22-rdf-syntax-ns#List" />
		<rdfs:subClassOf>
			<owl:Restriction>
				<owl:onProperty rdf:resource="http://www.w3.org/1999/02/22-rdf-syntax-ns#first" />
				<owl:allValuesFrom rdf:resource="http://dkm.fbk.eu/springles/ruleset#ClosureTask" />
			</owl:Restriction>
		</rdfs:subClassOf>
		<rdfs:subClassOf>
			<owl:Restriction>
				<owl:onProperty rdf:resource="http://www.w3.org/1999/02/22-rdf-syntax-ns#rest" />
				<owl:allValuesFrom rdf:resource="http://dkm.fbk.eu/springles/ruleset#ClosureTaskList" />
			</owl:Restriction>
		</rdfs:subClassOf>
	</owl:Class>
	<owl:DatatypeProperty rdf:about="http://dkm.fbk.eu/springles/ruleset#bind">
		<rdfs:label xml:lang="en">bind</rdfs:label>
		<rdfs:comment xml:lang="en">Declares a binding for the subject closure task. The value
        is binding is a string of the form 'variable = SPARQL expression'. The
        expression is evaluated only on the basis of inherited bindings.</rdfs:comment>
		<rdfs:domain rdf:resource="http://dkm.fbk.eu/springles/ruleset#ClosureTask" />
		<rdfs:range rdf:resource="http://www.w3.org/2001/XMLSchema#string" />
	</owl:DatatypeProperty>
	<owl:Class rdf:about="http://dkm.fbk.eu/springles/ruleset#ClosureEvalTask">
		<rdfs:label xml:lang="en">closure eval task</rdfs:label>
		<rdfs:comment xml:lang="en">A closure task consisting in the evaluation of zero or more
        rules, specified using mandatory property
        &lt;a href='#evalOf'&gt;spr:evalOf&lt;/a&gt;.</rdfs:comment>
		<rdfs:subClassOf rdf:resource="http://dkm.fbk.eu/springles/ruleset#ClosureTask" />
		<rdfs:subClassOf>
			<owl:Restriction>
				<owl:onProperty>
					<owl:ObjectProperty rdf:about="http://dkm.fbk.eu/springles/ruleset#evalOf">
						<rdf:type rdf:resource="http://www.w3.org/2002/07/owl#FunctionalProperty" />
						<rdfs:label xml:lang="en">evaluation of</rdfs:label>
						<rdfs:comment xml:lang="en">Specifies the list of rules to be evaluated in parallel as
        part of the execution of a
        &lt;a href='#ClosureEvalTask'&gt;spr:ClosureEvalTask&lt;/a&gt;.</rdfs:comment>
						<rdfs:domain rdf:resource="http://dkm.fbk.eu/springles/ruleset#ClosureEvalTask" />
						<rdfs:range rdf:resource="http://dkm.fbk.eu/springles/ruleset#RuleList" />
					</owl:ObjectProperty>
				</owl:onProperty>
				<owl:minCardinality rdf:datatype="http://www.w3.org/2001/XMLSchema#nonNegativeInteger">1</owl:minCardinality>
			</owl:Restriction>
		</rdfs:subClassOf>
	</owl:Class>
	<owl:Class rdf:about="http://dkm.fbk.eu/springles/ruleset#ClosureSequenceTask">
		<rdfs:label xml:lang="en">closure sequence task</rdfs:label>
		<rdfs:comment xml:lang="en">A closure task consisting in the sequential execution of
        zero or more child tasks, specified using mandatory property
        &lt;a href='#sequenceOf'&gt;spr:sequenceOf&lt;/a&gt;.</rdfs:comment>
		<rdfs:subClassOf rdf:resource="http://dkm.fbk.eu/springles/ruleset#ClosureTask" />
		<rdfs:subClassOf>
			<owl:Restriction>
				<owl:onProperty>
					<owl:ObjectProperty rdf:about="http://dkm.fbk.eu/springles/ruleset#sequenceOf">
						<rdf:type rdf:resource="http://www.w3.org/2002/07/owl#FunctionalProperty" />
						<rdfs:label xml:lang="en">sequence of</rdfs:label>
						<rdfs:comment xml:lang="en">Specifies the list of child tasks to be executed
        sequentially as part of the execution of a
        &lt;a href='#ClosureSequenceTask'&gt;spr:ClosureSequenceTask&lt;/a&gt;.</rdfs:comment>
						<rdfs:domain rdf:resource="http://dkm.fbk.eu/springles/ruleset#ClosureSequenceTask" />
						<rdfs:range rdf:resource="http://dkm.fbk.eu/springles/ruleset#ClosureTaskList" />
					</owl:ObjectProperty>
				</owl:onProperty>
				<owl:minCardinality rdf:datatype="http://www.w3.org/2001/XMLSchema#nonNegativeInteger">1</owl:minCardinality>
			</owl:Restriction>
		</rdfs:subClassOf>
	</owl:Class>
	<owl:Class rdf:about="http://dkm.fbk.eu/springles/ruleset#ClosureFixPointTask">
		<rdfs:label xml:lang="en">closure fix-point task</rdfs:label>
		<rdfs:comment xml:lang="en">A closure task consisting in the fix-point execution of a
        child task, specified using mandatory property
        &lt;a href='#fixPointOf'&gt;spr:fixPointOf&lt;/a&gt;.</rdfs:comment>
		<rdfs:subClassOf rdf:resource="http://dkm.fbk.eu/springles/ruleset#ClosureTask" />
		<rdfs:subClassOf>
			<owl:Restriction>
				<owl:onProperty>
					<owl:ObjectProperty rdf:about="http://dkm.fbk.eu/springles/ruleset#fixPointOf">
						<rdf:type rdf:resource="http://www.w3.org/2002/07/owl#FunctionalProperty" />
						<rdfs:label xml:lang="en">fix-point of</rdfs:label>
						<rdfs:comment xml:lang="en">Specifies the sub-task to be executed in a fix-point mode
        as part of the execution of a
        &lt;a href='#ClosureFixPointTask'&gt;spr:ClosureFixPointTask&lt;/a&gt;.</rdfs:comment>
						<rdfs:domain rdf:resource="http://dkm.fbk.eu/springles/ruleset#ClosureFixPointTask" />
						<rdfs:range rdf:resource="http://dkm.fbk.eu/springles/ruleset#ClosureTask" />
					</owl:ObjectProperty>
				</owl:onProperty>
				<owl:minCardinality rdf:datatype="http://www.w3.org/2001/XMLSchema#nonNegativeInteger">1</owl:minCardinality>
			</owl:Restriction>
		</rdfs:subClassOf>
	</owl:Class>
	<owl:Class rdf:about="http://dkm.fbk.eu/springles/ruleset#ClosureRepeatTask">
		<rdfs:label xml:lang="en">closure repeat task</rdfs:label>
		<rdfs:comment xml:lang="en">A closure task consisting in the repeated execution of a
        child task, specified by property &lt;a href='#repeatOf'&gt;spr:repeatOf&lt;/a&gt;,
        for each tuple obtained from the evaluation of a &lt;code&gt;SELECT&lt;/code&gt;
        query, specified by property
        &lt;a href='#repeatOver'&gt;spr:repeatOver&lt;/a&gt;.</rdfs:comment>
		<rdfs:subClassOf rdf:resource="http://dkm.fbk.eu/springles/ruleset#ClosureTask" />
		<rdfs:subClassOf>
			<owl:Restriction>
				<owl:onProperty>
					<owl:ObjectProperty rdf:about="http://dkm.fbk.eu/springles/ruleset#repeatOf">
						<rdf:type rdf:resource="http://www.w3.org/2002/07/owl#FunctionalProperty" />
						<rdfs:label xml:lang="en">repeat of</rdfs:label>
						<rdfs:comment xml:lang="en">Specifies the sub-task to be repeatedly executed as part of
        the execution of a
        &lt;a href='#ClosureRepeatTask'&gt;spr:ClosureRepeatTask&lt;/a&gt;.</rdfs:comment>
						<rdfs:domain rdf:resource="http://dkm.fbk.eu/springles/ruleset#ClosureRepeatTask" />
						<rdfs:range rdf:resource="http://dkm.fbk.eu/springles/ruleset#ClosureTask" />
					</owl:ObjectProperty>
				</owl:onProperty>
				<owl:minCardinality rdf:datatype="http://www.w3.org/2001/XMLSchema#nonNegativeInteger">1</owl:minCardinality>
			</owl:Restriction>
		</rdfs:subClassOf>
		<rdfs:subClassOf>
			<owl:Restriction>
				<owl:onProperty>
					<owl:DatatypeProperty rdf:about="http://dkm.fbk.eu/springles/ruleset#repeatOver">
						<rdf:type rdf:resource="http://www.w3.org/2002/07/owl#FunctionalProperty" />
						<rdfs:label xml:lang="en">repeat over</rdfs:label>
						<rdfs:comment xml:lang="en">Specifies the query whose results control the execution of a
        child task in a
        &lt;a href='#ClosureRepeatTask'&gt;spr:ClosureRepeatTask&lt;/a&gt;.</rdfs:comment>
						<rdfs:domain rdf:resource="http://dkm.fbk.eu/springles/ruleset#ClosureRepeatTask" />
						<rdfs:range rdf:resource="http://www.w3.org/2001/XMLSchema#string" />
					</owl:DatatypeProperty>
				</owl:onProperty>
				<owl:minCardinality rdf:datatype="http://www.w3.org/2001/XMLSchema#nonNegativeInteger">1</owl:minCardinality>
			</owl:Restriction>
		</rdfs:subClassOf>
	</owl:Class>
	<owl:AllDisjointClasses>
		<owl:members>
			<rdf:Description>
				<rdf:first rdf:resource="http://dkm.fbk.eu/springles/ruleset#ClosureEvalTask" />
				<rdf:rest>
					<rdf:Description>
						<rdf:first rdf:resource="http://dkm.fbk.eu/springles/ruleset#ClosureSequenceTask" />
						<rdf:rest>
							<rdf:Description>
								<rdf:first rdf:resource="http://dkm.fbk.eu/springles/ruleset#ClosureFixPointTask" />
								<rdf:rest>
									<rdf:Description>
										<rdf:first rdf:resource="http://dkm.fbk.eu/springles/ruleset#ClosureRepeatTask" />
										<rdf:rest rdf:resource="http://www.w3.org/1999/02/22-rdf-syntax-ns#nil" />
									</rdf:Description>
								</rdf:rest>
							</rdf:Description>
						</rdf:rest>
					</rdf:Description>
				</rdf:rest>
			</rdf:Description>
		</owl:members>
	</owl:AllDisjointClasses>
	<owl:AllDisjointClasses>
		<owl:members>
			<rdf:Description>
				<rdf:first rdf:resource="http://dkm.fbk.eu/springles/ruleset#Ruleset" />
				<rdf:rest>
					<rdf:Description>
						<rdf:first rdf:resource="http://dkm.fbk.eu/springles/ruleset#Parameter" />
						<rdf:rest>
							<rdf:Description>
								<rdf:first rdf:resource="http://dkm.fbk.eu/springles/ruleset#Rule" />
								<rdf:rest>
									<rdf:Description>
										<rdf:first rdf:resource="http://dkm.fbk.eu/springles/ruleset#RuleList" />
										<rdf:rest>
											<rdf:Description>
												<rdf:first rdf:resource="http://dkm.fbk.eu/springles/ruleset#ClosureTask" />
												<rdf:rest>
													<rdf:Description>
														<rdf:first rdf:resource="http://dkm.fbk.eu/springles/ruleset#ClosureTaskList" />
														<rdf:rest rdf:resource="http://www.w3.org/1999/02/22-rdf-syntax-ns#nil" />
													</rdf:Description>
												</rdf:rest>
											</rdf:Description>
										</rdf:rest>
									</rdf:Description>
								</rdf:rest>
							</rdf:Description>
						</rdf:rest>
					</rdf:Description>
				</rdf:rest>
			</rdf:Description>
		</owl:members>
	</owl:AllDisjointClasses>
</rdf:RDF>